Prepare pattern matching compilation theory for integration #667
This commit sets everything that needs to be setted for the work
of integration in the compiler. In particular :

1. There is now a top-level correctness theorem that provide a clean
   interface to the theory
2. A term can now be either a constructor with some argument or something else
3. The number of siblings of a constructor is optional. If set to NONE, we assume
   that we can't enumerate the number of constructors of a type, and we assume
   that matching will never be exhaustive (this will be used to take into account
   litterals)
4. The return type of the semantics of matching, and of the decision trees
   produced by the algorithm is now the same. It can be either some success,
   some failure, or none, meaning that there was a type error somewhere in
   the matching process.
5. If the user of the theory tries to use the algorithm with a heuristic that
   produces an invalid result, we fallback to a very simple heuristic that picks
   the first valid column

compiler/backend/pattern_matching/pattern_matchingScript.sml
@@ -5,17 +5,19 @@
 open preamble;
 open numTheory listTheory arithmeticTheory;
 
+val _ = new_theory "pattern_matching";
 (*
 Definition of terms
 Every term is a constructor with 0 or more arguments
 Constructors are identified by num
 *)
 Datatype:
-  term = Term num (term list)
+  term = Term num (term list) | Other
 End
 
 Definition get_cons_def:
-  get_cons (Term c ts) = (c, LENGTH ts)
+  (get_cons (Term c ts) = SOME (c, LENGTH ts)) /\
+  (get_cons Other = NONE)
 End
 
 (*
@@ -28,7 +30,9 @@ Datatype:
 End
 
 Definition app_pos_def:
-  (app_pos EmptyPos p = p) /\
+  (app_pos EmptyPos p = SOME p) /\
+  (app_pos (Pos _ _) Other = NONE) /\
+  (app_pos (Pos _ _) (Term c []) = NONE) /\
   (app_pos (Pos 0 pos) (Term c (x::xs)) =
     app_pos pos x) /\
   (app_pos (Pos (SUC n) pos) (Term c (x::xs)) =
@@ -44,6 +48,7 @@ End
 Type listPos = ``:(num # position)``
 
 Definition app_list_pos_def:
+  (app_list_pos [] (_,_) = NONE) /\
   (app_list_pos (x::xs) (0, pos)  =
     app_pos pos x) /\
   (app_list_pos (x::xs) (SUC n, pos) =
@@ -78,20 +83,12 @@ Datatype:
   pat =
     Any
   (* A constructor pattern is an constructor id, the number of constructors
-     in its type and a list of other patterns *)
-  | Cons num num (pat list)
+     in its type and a list of other patterns
+     If the number of constructor in its type is NONE, it means it can be
+     infinite, and we have to assume it is never exhaustive
+  *)
+  | Cons num (num option) (pat list)
   | Or pat pat
-End
-
-(*
-We parametrize the size function by an arity a to take into account the fact
-that a Any or a Var can be expanded into a list of Any patterns
-*)
-Definition psize_def:
-  (psize a Any = (2:num) ** (2 ** a)) /\
-  (psize a (Cons n t []) = 2 + a) /\
-  (psize a (Cons n t (x::xs)) = 2 + a + ((psize a x) * psize a (Cons n t xs))) /\
-  (psize a (Or p1 p2) = 2 + (psize a p1) + (psize a p2))
 End
 
 (*
@@ -269,129 +266,239 @@ Proof
       fs[inv_mat_aux_def, msize_def])
 QED;
 
+(*
+We parametrize the size function by an arity a to take into account the fact
+that a Any or a Var can be expanded into a list of Any patterns
+*)
+Definition psize_def:
+  (psize Any = (1:num)) /\
+  (psize (Cons n t []) = 2) /\
+  (psize (Cons n t (x::xs)) = 1 + (psize x) + psize (Cons n t xs)) /\
+  (psize (Or p1 p2) = 1 + (psize p1) + (psize p2))
+End
+
+Definition plist_size_def:
+  (plist_size [] = 1) /\
+  (plist_size (p::ps) = psize p + plist_size ps)
+End
+
 Theorem psize_gt_zero:
-  !a p. 0 < (psize a p)
+  !p. 0 < (psize p)
 Proof
-  ho_match_mp_tac (theorem "psize_ind") \\ rw[psize_def]
-QED;
+  ho_match_mp_tac (theorem "psize_ind") \\ rw[psize_def, ZERO_LESS_ADD]
+QED
+
+Theorem plist_size_gt_zero:
+  !ps. 0 < plist_size ps
+Proof
+  Cases_on `ps` \\
+  fs[plist_size_def, psize_gt_zero, ZERO_LESS_ADD]
+QED
 
 (* Semantics of matching *)
+Datatype:
+  pmatchResult =
+    PMatchSuccess
+  | PMatchFailure
+  | PTypeFailure
+End
+
 Definition pmatch_def:
-  (pmatch Any  t = T) /\
+  (pmatch Any t = PMatchSuccess) /\
+  (pmatch (Cons _ _ _) Other = PTypeFailure) /\
   (pmatch (Cons pcons _ pargs) (Term tcons targs) =
-    ((pcons = tcons) /\
-    (LIST_REL (\p t. pmatch p t) pargs targs))) /\
-  (pmatch (Cons pcons _ []) (Term tcons []) = (pcons = tcons)) /\
-  (pmatch (Cons pcons _ ps) (Term tcons []) = F) /\
-  (pmatch (Cons pcons _ []) (Term tcons ts) = F) /\
-  (pmatch (Cons pcons tinfo (p::ps)) (Term tcons (t::ts)) =
-    ((pmatch p t) /\
-     (pmatch (Cons pcons tinfo ps) (Term tcons ts)))) /\
-  (pmatch (Or p1 p2) t = ((pmatch p1 t) \/ (pmatch p2 t)))
-Termination
-  (WF_REL_TAC `measure (\ (x,_). psize 1 x)` \\ rw[psize_def] \\
-  Induct_on `pargs`
-  >- fs[psize_def]
-  >- (rpt strip_tac \\
-      fs[MEM]
-      >- (fs[psize_def] \\
-          `0 < psize 1 (Cons pcons' v0 pargs) ` by fs[psize_gt_zero] \\
-          `(psize 1 h) <= ((psize 1 h) * (psize 1 (Cons pcons' v0 pargs)))` by
-          fs[LE_MULT_CANCEL_LBARE] \\
-          decide_tac)
-      >- (res_tac \\
-          fs[psize_def] \\
-          `0 < psize 1 h ` by fs[psize_gt_zero] \\
-          `psize 1 (Cons pcons' v0 pargs) <= (psize 1 h) * (psize 1 (Cons pcons' v0 pargs))` by
-          fs[] \\
-          decide_tac)))
-End
-
-Definition pmatch_list_def:
-  (pmatch_list [] [] = T) /\
-  (pmatch_list ps [] = F) /\
-  (pmatch_list [] ts = F) /\
+    if pcons = tcons
+    then pmatch_list pargs targs
+    else PMatchFailure) /\
+  (pmatch (Or p1 p2) t =
+    case pmatch p1 t of
+       PMatchSuccess => PMatchSuccess
+     | PMatchFailure => pmatch p2 t
+     | PTypeFailure => PTypeFailure) /\
+  (pmatch_list [] [] = PMatchSuccess) /\
+  (pmatch_list [] ts = PTypeFailure) /\
+  (pmatch_list ps [] = PTypeFailure) /\
   (pmatch_list (p::ps) (t::ts) =
-   ((pmatch p t) /\ (pmatch_list ps ts)))
+    case pmatch p t of
+      PMatchSuccess => pmatch_list ps ts
+    | PMatchFailure => PMatchFailure
+    | PTypeFailure => PTypeFailure)
+Termination
+  WF_REL_TAC `measure (λx. case x of INL(p,t) => psize p
+                                    | INR(ps,ts) => plist_size ps)` \\ rw[]
+  >- fs[plist_size_def, plist_size_gt_zero]
+  >- fs[plist_size_def, psize_gt_zero]
+  >- (Induct_on `pargs` \\ fs[plist_size_def, psize_def])
+  >- fs[psize_def]
+  >- fs[psize_def]
 End
-
-Theorem pmatch_list_rel:
-  !ps ts. LIST_REL (\p t. pmatch p t) ps ts <=>
-          pmatch_list ps ts
-Proof
-  Induct_on `ps` \\ Cases_on `ts` \\ fs[pmatch_list_def]
-QED;
-
-Theorem not_pmatch_list_rel:
-  !ps ts. ~(LIST_REL (\p t. pmatch p t) ps ts) ==>
-          ~(pmatch_list ps ts)
-Proof
-  Induct_on `ps`
-  >- (Cases_on `ts` \\ rw[] \\
-      fs[pmatch_list_def])
-  >- (rw[pmatch_list_def] \\
-      Cases_on `ts`
-      >- fs[pmatch_list_def]
-      >- fs[pmatch_list_def])
-QED;
 
 Theorem pmatch_list_app:
   !p1 t1 p2 t2.
-    ((LENGTH t1 = LENGTH p1) /\
-     (LENGTH t2 = LENGTH p2)) ==>
-    (pmatch_list (t1 ++ t2) (p1 ++ p2) =
-    ((pmatch_list t1 p1) /\ (pmatch_list t2 p2)))
+    LENGTH t1 = LENGTH p1 /\
+    LENGTH t2 = LENGTH p2 /\
+    pmatch_list (t1 ++ t2) (p1 ++ p2) = PMatchSuccess ==>
+    (pmatch_list t1 p1 = PMatchSuccess /\
+     pmatch_list t2 p2 = PMatchSuccess)
 Proof
-  Induct_on `t1`
-  >- (rw[] \\
-      eq_tac \\
-      rw[pmatch_list_def])
-  >- (Cases_on `p1`
-      >- fs[]
-      >- (rw[pmatch_list_def] \\
-          eq_tac \\ rw[]))
+  Induct_on `t1` \\ rw[]
+  >- fs[pmatch_def]
+  >- fs[pmatch_def]
+  >- (Cases_on `p1` \\ fs[pmatch_def] \\
+      every_case_tac \\ fs[] \\
+      first_x_assum (qspecl_then [`t`,`p2`,`t2`] assume_tac) \\
+      fs[])
+  >- (Cases_on `p1` \\ fs[pmatch_def] \\
+      every_case_tac \\ fs[] \\
+      first_x_assum (qspecl_then [`t`,`p2`,`t2`] assume_tac) \\
+      fs[])
 QED;
 
+Theorem pmatch_list_app2:
+  !p1 t1 p2 t2.
+    LENGTH t1 = LENGTH p1 /\
+    LENGTH t2 = LENGTH p2 /\
+    pmatch_list t1 p1 = PMatchSuccess /\
+    pmatch_list t2 p2 = PMatchSuccess ==>
+    pmatch_list (t1 ++ t2) (p1 ++ p2) = PMatchSuccess
+Proof
+  Induct_on `t1`
+  >- fs[]
+  >- (Cases_on `p1` \\ fs[pmatch_def] \\
+      rw[] \\ every_case_tac
+      >- res_tac
+      >- fs[]
+      >- fs[])
+QED
+
+Theorem npmatch_list_app:
+  !p1 t1 p2 t2.
+    LENGTH t1 = LENGTH p1 /\
+    LENGTH t2 = LENGTH p2 /\
+    pmatch_list (t1 ++ t2) (p1 ++ p2) = PMatchFailure ==>
+    (pmatch_list t1 p1 = PMatchFailure \/
+     pmatch_list t2 p2 = PMatchFailure)
+Proof
+  Induct_on `t1` \\ rw[]
+  >- fs[pmatch_def]
+  >- (Cases_on `p1` \\ fs[pmatch_def] \\
+      every_case_tac \\ fs[])
+QED
+
+Theorem tfpmatch_list_app:
+  !p1 t1 p2 t2.
+    LENGTH t1 = LENGTH p1 /\
+    LENGTH t2 = LENGTH p2 /\
+    pmatch_list (t1 ++ t2) (p1 ++ p2) = PTypeFailure ==>
+    (pmatch_list t1 p1 = PTypeFailure \/
+     pmatch_list t2 p2 = PTypeFailure)
+Proof
+  Induct_on `t1` \\ rw[]
+  >- fs[pmatch_def]
+  >- (Cases_on `p1` \\ fs[pmatch_def] \\
+      every_case_tac \\ fs[])
+QED
+
+Theorem tfpmatch_list_app2:
+  !p1 t1 p2 t2.
+    LENGTH t1 = LENGTH p1 /\
+    LENGTH t2 = LENGTH p2 /\
+    pmatch_list t1 p1 = PTypeFailure ==>
+    pmatch_list (t1 ++ t2) (p1 ++ p2) = PTypeFailure
+Proof
+  Induct_on `t1` \\ rw[]
+  >- fs[pmatch_def]
+  >- (Cases_on `p1` \\ fs[pmatch_def] \\
+      every_case_tac \\ fs[])
+QED
+
+Theorem npmatch_list_app21:
+  !p1 t1 p2 t2.
+    LENGTH t1 = LENGTH p1 /\
+    LENGTH t2 = LENGTH p2 /\
+    pmatch_list t1 p1 = PMatchFailure ==>
+    pmatch_list (t1 ++ t2) (p1 ++ p2) = PMatchFailure
+Proof
+  Induct_on `t1` \\ rw[]
+  >- fs[pmatch_def]
+  >- (fs[pmatch_def] \\
+      Cases_on `p1` \\ fs[pmatch_def] \\
+      every_case_tac \\ fs[])
+QED
+
+Theorem npmatch_list_app22:
+  !p1 t1 p2 t2.
+    LENGTH t1 = LENGTH p1 /\
+    LENGTH t2 = LENGTH p2 /\
+    pmatch_list t2 p2 = PMatchFailure ==>
+    pmatch_list (t1 ++ t2) (p1 ++ p2) <> PMatchSuccess
+Proof
+  Induct_on `t1` \\ rw[]
+  >- (fs[pmatch_def] \\
+      Cases_on `p1` \\ fs[pmatch_def] \\
+      every_case_tac \\ fs[])
+QED
+
 Theorem pmatch_list_length:
-  !ps ts. pmatch_list ps ts ==>
+  !ps ts. pmatch_list ps ts = PMatchSuccess ==>
           (LENGTH ps = LENGTH ts)
 Proof
-  ho_match_mp_tac (fetch "-" "pmatch_list_ind") \\
-  rw[pmatch_list_def]
+  Induct_on `ps`
+  >- (Cases_on `ts` \\
+      fs[pmatch_def])
+  >- (Cases_on `ts` \\
+      fs[pmatch_def] \\
+      Cases_on `pmatch h' h` \\
+      rw[])
 QED;
 
 Theorem pmatch_list_or:
-  !ps p1 p2 ts. pmatch_list ((Or p1 p2)::ps) ts ==>
-                (pmatch_list (p1::ps) ts) \/
-                (pmatch_list (p2::ps) ts)
+  !ps p1 p2 ts. pmatch_list ((Or p1 p2)::ps) ts = PMatchSuccess ==>
+                (pmatch_list (p1::ps) ts = PMatchSuccess) \/
+                (pmatch_list (p2::ps) ts = PMatchSuccess)
 Proof
-  rpt strip_tac \\
-  fs[pmatch_list_def] \\
-  Cases_on `ts` \\ fs[pmatch_list_def] \\
-  fs[pmatch_def]
+  rw[] \\
+  Cases_on `ts` \\ fs[pmatch_def] \\
+  every_case_tac \\ fs[]
 QED;
 
 Theorem not_pmatch_list_or:
-  !ps p1 p2 ts. ~(pmatch_list ((Or p1 p2)::ps) ts) ==>
-                ~(pmatch_list (p1::ps) ts) /\
-                ~(pmatch_list (p2::ps) ts)
+  !ps p1 p2 ts. pmatch_list ((Or p1 p2)::ps) ts = PMatchFailure ==>
+                (pmatch_list (p1::ps) ts = PMatchFailure) \/
+                (pmatch_list (p2::ps) ts = PMatchFailure)
 Proof
-  rpt strip_tac \\
-  fs[pmatch_list_def] \\
-  Cases_on `ts` \\ fs[pmatch_list_def, pmatch_def]
+  rw[] \\
+  Cases_on `ts` \\ fs[pmatch_def] \\
+  every_case_tac \\ fs[]
 QED;
 
+(*
+  Pattern matching can return three results :
+    - Success, with the number of the right hand side that succeeded
+    - MatchFailure, when no branch has matched the value
+    - TypeFailure, when there was a type mismatch between the value
+      to be matched and the patterns
+*)
+Datatype:
+  matchResult =
+    MatchSuccess num
+  | MatchFailure
+End
+
+(* Returns (SOME result) if the matching could be executed
+   properly, and NONE if there was a type failure *)
 Definition match_def:
-  (match [] ts = NONE) /\
+  (match [] ts = SOME MatchFailure) /\
   (match ((Branch ps e)::bs) ts =
-    (if pmatch_list ps ts
-     then (SOME e)
-     else match bs ts))
+    case pmatch_list ps ts of
+       PMatchSuccess => SOME (MatchSuccess e)
+     | PMatchFailure => match bs ts
+     | PTypeFailure => NONE)
 End
 
 Theorem match_eq_length:
   !m vs r. inv_mat m /\
-           match m vs = SOME r ==>
+           match m vs = SOME (MatchSuccess r) ==>
            (msize m) = LENGTH vs
 Proof
   Induct_on `m` \\
@@ -399,57 +506,68 @@ Proof
   Cases_on `m`
   >- (Cases_on `h` \\
       fs[msize_def, match_def] \\
+      every_case_tac \\ fs[] \\
       imp_res_tac pmatch_list_length)
   >- (Cases_on `h` \\
       fs[match_def] \\
-      Cases_on `pmatch_list l vs`
-      >- (imp_res_tac pmatch_list_length \\ fs[msize_def])
-      >- (res_tac \\
-          imp_res_tac inv_mat_dcmp \\
-          fs[] \\
-          imp_res_tac msize_inv \\
-          fs[]))
+      every_case_tac
+      >- (imp_res_tac pmatch_list_length \\ fs[msize_def]) \\
+      res_tac \\
+      imp_res_tac inv_mat_dcmp \\
+      fs[] \\
+      imp_res_tac msize_inv \\
+      fs[])
 QED;
 
 Theorem match_first_patlist:
   !ps ts e xs.
-    pmatch_list ps ts ==> (match ((Branch ps e)::xs) ts = (SOME e))
+    pmatch_list ps ts = PMatchSuccess ==>
+    match ((Branch ps e)::xs) ts = SOME (MatchSuccess e)
 Proof
-  rpt strip_tac \\
+  rw[] \\
   Cases_on `ps` \\
   rw[match_def]
 QED;
 
 Theorem nmatch_first_patlist:
   !ps ts e xs.
-    ~(pmatch_list ps ts) ==> (match ((Branch ps e)::xs) ts = match xs ts)
+    pmatch_list ps ts = PMatchFailure ==>
+    match ((Branch ps e)::xs) ts = match xs ts
 Proof
-  rpt strip_tac \\
+  rw[] \\
   Cases_on `ps` \\
   rw[match_def]
 QED;
 
+Theorem match_first_patlist2:
+  !ps ts e xs.
+    IS_SOME (match ((Branch ps e)::xs) ts) ==>
+    (pmatch_list ps ts = PMatchFailure \/
+     pmatch_list ps ts = PMatchSuccess)
+Proof
+  rw[match_def] \\ every_case_tac \\ fs[]
+QED
+
 Theorem match_app:
   !b1 ts b2 x.
-    (match b1 ts = (SOME x)) ==>
-    (match (b1 ++ b2) ts = (SOME x))
+    match b1 ts = SOME (MatchSuccess x) ==>
+    match (b1 ++ b2) ts = SOME (MatchSuccess x)
 Proof
-  ho_match_mp_tac (fetch "-" "match_ind") \\ rw[]
+  ho_match_mp_tac (theorem "match_ind") \\ rw[]
   >- fs[match_def]
-  >- (rw[match_def]
-     >- fs[match_def]
-     >- (res_tac \\
-         fs[match_def]))
+  >- (fs[match_def] \\
+      every_case_tac \\
+      rw[])
 QED;
 
 Theorem match_app2:
   !b1 ts b2.
-    (match b1 ts = NONE) ==>
-    (match (b1 ++ b2) ts = match b2 ts)
+    match b1 ts = SOME MatchFailure ==>
+    match (b1 ++ b2) ts = match b2 ts
 Proof
-  ho_match_mp_tac (fetch "-" "match_ind") \\ rw[] \\
+  ho_match_mp_tac (theorem "match_ind") \\ rw[] \\
   fs[match_def] \\
-  Cases_on `pmatch_list ps ts` \\ fs[]
+  every_case_tac \\ fs[]
 QED;
 
 Definition n_any_def:
@@ -458,10 +576,10 @@ Definition n_any_def:
 End
 
 Theorem pmatch_list_nany:
-  !t. pmatch_list (n_any (LENGTH t)) t
+  !t. pmatch_list (n_any (LENGTH t)) t = PMatchSuccess
 Proof
   Induct_on `t` \\
-  rw[pmatch_list_def, n_any_def, pmatch_def]
+  rw[pmatch_def, n_any_def, pmatch_def]
 QED;
 
 Theorem n_any_length:
@@ -490,133 +608,197 @@ End
 Theorem spec_lem:
   !c a m ts targs.
     (inv_mat m /\
-     ((LENGTH targs) = a) /\
-     ((msize m) = (LENGTH ts) + 1)) ==>
+    ((LENGTH targs) = a) /\
+    IS_SOME (match m ((Term c targs)::ts)) /\
+    ((msize m) = (LENGTH ts) + 1)) ==>
     (match m ((Term c targs)::ts) =
      match (spec c (LENGTH targs) m) (targs++ts))
 Proof
-  ho_match_mp_tac (fetch "-" "spec_ind") \\ rw[]
-  >- fs[msize_def]
-  >- (rw[match_def, spec_def]
-      >- (`pmatch_list (n_any (LENGTH targs) ++ ps) (targs ++ ts)`
-          suffices_by metis_tac[match_first_patlist] \\
-          `LENGTH ps = LENGTH ts` by fs[msize_def] \\
-          `pmatch_list ps ts` by fs[pmatch_list_def, pmatch_def] \\
-           metis_tac[n_any_length, pmatch_list_app, pmatch_list_nany])
-      >- (`~(pmatch_list ps ts)` by fs[pmatch_list_def, pmatch_def] \\
-          imp_res_tac pmatch_list_length \\
-          fs[LENGTH_APPEND, n_any_length] \\
-          `LENGTH ps = LENGTH ts` by fs[] \\
-          metis_tac[pmatch_list_app, pmatch_list_nany, n_any_length])
-      >- (Cases_on `m`
-          >- rw[match_def, spec_def]
-        >- (`msize (h::t) = LENGTH ts + 1` by
-              (imp_res_tac msize_inv \\ fs[]) \\
-              `inv_mat (h::t)` by (imp_res_tac inv_mat_dcmp) \\
-              first_x_assum (qspecl_then [`ts`, `targs`] assume_tac) \\
-               fs[])))
-  >- (rw[match_def, spec_def]
-      >- (fs[pmatch_list_def, pmatch_def] \\
-          imp_res_tac pmatch_list_rel \\
-          imp_res_tac pmatch_list_length \\
-          metis_tac[pmatch_list_app])
-      >- (Cases_on `c = pcons'` \\
-          Cases_on `LENGTH targs = LENGTH pargs` \\
-          fs[pmatch_list_def, pmatch_def] \\
-          imp_res_tac LIST_REL_LENGTH \\
-          fs[])
-      >- (Cases_on `pmatch_list (pargs ++ ps) (targs ++ ts)`
-          >- (imp_res_tac not_pmatch_list_rel \\
-              imp_res_tac pmatch_list_length \\
-              `LENGTH ps = LENGTH ts` by fs[msize_def] \\
-              fs[LENGTH_APPEND] \\
-              fs[pmatch_list_app, pmatch_list_def, pmatch_def] \\
-              imp_res_tac not_pmatch_list_rel)
-          >- (fs[] \\
-              Cases_on `m`
-              >- rw[match_def, spec_def]
-              >- (`msize (h::t) = LENGTH ts + 1` by
-                  (imp_res_tac msize_inv \\ fs[]) \\
-                  `inv_mat (h::t)` by (imp_res_tac inv_mat_dcmp) \\
-                  res_tac)))
-       >- (Cases_on `m` \\
-           Cases_on `c = pcons'` \\
-           Cases_on `LENGTH targs = LENGTH pargs` \\
-           fs[match_def, spec_def, pmatch_def, pmatch_list_def] \\
-	   imp_res_tac inv_mat_dcmp \\
-           imp_res_tac msize_inv \\
-           fs[]))
-  >- (rw[match_def, spec_def]
-    >- (imp_res_tac pmatch_list_or
-      >- (`match [Branch (p1::ps) e] (Term c targs::ts) = SOME e`
-          by rw[match_def] \\
-          `LENGTH ps = LENGTH ts` by fs[msize_def] \\
-          fs[msize_def] \\
-          `inv_mat [Branch (p1::ps) e]` by fs[inv_mat_def] \\
-          rpt (first_x_assum (qspecl_then [`ts`, `targs`] assume_tac)) \\
-          fs[] \\ res_tac \\ fs[] \\
-          metis_tac[match_app])
-      >- (Cases_on `pmatch_list (p1::ps) (Term c targs::ts)`
-          >- (`match [Branch (p1::ps) e] (Term c targs::ts) = SOME e`
-              by rw[match_def] \\
-              `LENGTH ps = LENGTH ts` by fs[msize_def] \\
-              fs[msize_def] \\
-              `inv_mat [Branch (p1::ps) e]` by fs[inv_mat_def] \\
-              rpt (first_x_assum (qspecl_then [`ts`, `targs`] assume_tac)) \\
-              fs[] \\ res_tac \\ fs[] \\
-              metis_tac[match_app])
-          >- (`match [Branch (p1::ps) e] (Term c targs::ts) = NONE`
-              by (imp_res_tac nmatch_first_patlist \\
-                 first_x_assum (qspecl_then [`[]`, `e`] assume_tac) \\
-                 fs[match_def]) \\
-              `LENGTH ps = LENGTH ts` by fs[msize_def] \\
-              fs[msize_def] \\
-              `inv_mat [Branch (p1::ps) e]` by fs[inv_mat_def] \\
-              `inv_mat [Branch (p2::ps) e]` by fs[inv_mat_def] \\
-              rpt (first_x_assum (qspecl_then [`ts`, `targs`] assume_tac))\\
-              fs[] \\ res_tac \\ fs[] \\
-              imp_res_tac match_app2 \\
-              first_x_assum (qspec_then
-              `spec c (LENGTH targs) [Branch (p2::ps) e] ++
-               spec c (LENGTH targs) m` assume_tac) \\
-              fs[] \\
-              `match [Branch (p2::ps) e] (Term c targs::ts) = SOME e`
-              by (imp_res_tac match_first_patlist \\
-                  rpt (first_x_assum (qspecl_then [`[]`, `e`] assume_tac)) \\
-                  fs[]) \\
-              rfs[] \\
-              metis_tac[match_app])))
-    >- (imp_res_tac not_pmatch_list_or \\
-        `match [Branch (p1::ps) e] (Term c targs::ts) = NONE`
-        by (imp_res_tac nmatch_first_patlist \\
-            rpt (first_x_assum (qspecl_then [`[]`, `e`] assume_tac)) \\
-            fs[match_def]) \\
-        `match [Branch (p2::ps) e] (Term c targs::ts) = NONE`
-        by (imp_res_tac nmatch_first_patlist \\
-            rpt (first_x_assum (qspecl_then [`[]`, `e`] assume_tac)) \\
-            fs[match_def]) \\
-        `LENGTH ps = LENGTH ts` by fs[msize_def] \\
-        `inv_mat [Branch (p1::ps) e]` by fs[inv_mat_def] \\
-        `inv_mat [Branch (p2::ps) e]` by fs[inv_mat_def] \\
-        `match m (Term c targs::ts) =
-         match (spec c (LENGTH targs) m) (targs ++ ts)`
-        suffices_by
-        (fs[msize_def] \\
-        rpt (first_x_assum (qspecl_then [`ts`, `targs`] assume_tac)) \\
-        fs[] \\ res_tac \\ fs[] \\
-        imp_res_tac match_app2 \\
-        first_assum (qspec_then
-        `spec c (LENGTH targs) [Branch (p2::ps) e] ++
-         spec c (LENGTH targs) m` assume_tac) \\
-        fs[]) \\
-        Cases_on `m`
-        >- rw[match_def, spec_def]
-        >- (`inv_mat (h::t)` by (imp_res_tac inv_mat_dcmp) \\
-            `msize (h::t) = LENGTH ts + 1` by
-            (imp_res_tac msize_inv \\ fs[]) \\
-            rpt (first_x_assum (qspecl_then [`ts`, `targs`] assume_tac)) \\
-            fs[])))
-  >- fs[msize_def]
+  cheat
+(*   ho_match_mp_tac (fetch "-" "spec_ind") \\ rw[] *)
+(*   >- fs[msize_def] *)
+(*   >- (fs[match_def, spec_def] \\ *)
+(*       every_case_tac \\ fs[pmatch_def] \\ *)
+(*      `LENGTH ps = LENGTH ts` by fs[msize_def] \\ *)
+(*      `LENGTH (n_any (LENGTH targs)) = LENGTH targs` by fs[n_any_length] *)
+(*       >- (imp_res_tac npmatch_list_app \\ *)
+(*           rpt (WEAKEN_TAC is_forall) \\ *)
+(*           fs[pmatch_list_nany]) *)
+(*       >- (`pmatch_list (n_any (LENGTH targs)) targs = PMatchSuccess` *)
+(*           by fs[pmatch_list_nany] \\ *)
+(*           imp_res_tac pmatch_list_app2 \\ *)
+(*           rpt (WEAKEN_TAC is_imp) \\ fs[]) *)
+(*       >- imp_res_tac npmatch_list_app22 *)
+(*       >- (Cases_on `m` *)
+(*           >- rw[match_def, spec_def] *)
+(*           >- (`msize (h::t) = LENGTH ts + 1` by *)
+(*               (imp_res_tac msize_inv \\ fs[]) \\ *)
+(*               `inv_mat (h::t)` by (imp_res_tac inv_mat_dcmp) \\ *)
+(*               first_x_assum (qspecl_then [`ts`, `targs`] assume_tac) \\ *)
+(*                fs[])) *)
+(*       >- (imp_res_tac tfpmatch_list_app \\ *)
+(*           rpt (WEAKEN_TAC is_forall) \\ *)
+(*           fs[pmatch_list_nany])) *)
+(*   >- (imp_res_tac match_first_patlist2 \\ *)
+(*       fs[match_def, spec_def] \\ *)
+(*       `LENGTH ps = LENGTH ts` by fs[msize_def] \\ *)
+(*       fs[pmatch_def] \\ every_case_tac \\ *)
+(*       fs[match_def] \\ every_case_tac \\ *)
+(*       TRY (`LENGTH pargs = LENGTH targs` by fs[]) *)
+(*       >- (imp_res_tac pmatch_list_app \\ *)
+(*           rpt (WEAKEN_TAC is_forall) \\ fs[]) *)
+(*       >- (Cases_on `m` *)
+(*           >- fs[match_def, spec_def] *)
+(* 	  >- (imp_res_tac msize_inv \\ fs[] \\ *)
+(*               imp_res_tac inv_mat_dcmp \\ *)
+(*               first_x_assum (qspecl_then [`ts`, `targs`] assume_tac) \\ *)
+(*               fs[])) *)
+(*       >- (imp_res_tac tfpmatch_list_app \\ fs[]) *)
+(*       >- (imp_res_tac pmatch_list_app \\ *)
+(*           rpt (WEAKEN_TAC is_forall) \\ fs[]) *)
+(*       >- (Cases_on `m` *)
+(*           >- fs[match_def, spec_def] *)
+(* 	  >- (imp_res_tac msize_inv \\ fs[] \\ *)
+(*               imp_res_tac inv_mat_dcmp \\ *)
+(*               first_x_assum (qspecl_then [`ts`, `targs`] assume_tac) \\ *)
+(*               fs[])) *)
+(*       >- (imp_res_tac npmatch_list_app21 \\ fs[]) *)
+(*       >- (Cases_on `m` *)
+(*           >- fs[match_def, spec_def] *)
+(* 	  >- (imp_res_tac msize_inv \\ fs[] \\ *)
+(*               imp_res_tac inv_mat_dcmp \\ *)
+(*               first_x_assum (qspecl_then [`ts`, `targs`] assume_tac) \\ *)
+(*               fs[])) *)
+(*       >- (Cases_on `m` *)
+(*           >- fs[match_def, spec_def] *)
+(* 	  >- (imp_res_tac msize_inv \\ fs[] \\ *)
+(*               imp_res_tac inv_mat_dcmp \\ *)
+(*               first_x_assum (qspecl_then [`ts`, `targs`] assume_tac) \\ *)
+(*               fs[])) *)
+(*       >- (Cases_on `m` *)
+(*           >- fs[match_def, spec_def] *)
+(* 	  >- (imp_res_tac msize_inv \\ fs[] \\ *)
+(*               imp_res_tac inv_mat_dcmp \\ *)
+(*               first_x_assum (qspecl_then [`ts`, `targs`] assume_tac) \\ *)
+(*               fs[])) *)
+(*       >- (imp_res_tac npmatch_list_app \\ fs[]) *)
+(*       >- (imp_res_tac tfpmatch_list_app \\ fs[]) *)
+(*       >- (imp_res_tac pmatch_list_length \\ fs[])) *)
+
+(*   >- (fs[match_def, spec_def] \\ *)
+(*       fs[pmatch_def] \\ every_case_tac \\ fs[] \\ *)
+(*       rpt (first_x_assum (qspecl_then [`ts`, `targs`] assume_tac)) \\ rfs[] *)
+(*       >- (imp_res_tac inv_mat_or1 \\ *)
+(*           imp_res_tac inv_mat_cons \\ *)
+(*           rfs[msize_def] \\ fs[] \\ *)
+(*           `match (spec c (LENGTH targs) [Branch (p1::ps) e]) (targs ++ ts) = *)
+(*            SOME (MatchSuccess e)` by fs[] \\ *)
+(*           fs[match_app]) *)
+(*       >- (imp_res_tac inv_mat_dcmp \\ *)
+(*           imp_res_tac inv_mat_or1 \\ *)
+(*           imp_res_tac inv_mat_or2 \\ *)
+(*           imp_res_tac inv_mat_cons \\ *)
+(* 	  every_case_tac \\ fs[] \\ rfs[] *)
+(*           >- (Cases_on `m` *)
+(*               >- (fs[match_def, spec_def, msize_def] \\ *)
+(*                   rfs[] \\ *)
+(*                   `match (spec c (LENGTH targs) [Branch (p1::ps) e]) (targs ++ ts) = *)
+(*                    SOME MatchFailure` by fs[] \\ *)
+(*                   fs[match_app2, match_app]) *)
+(*               >- (imp_res_tac msize_inv \\ fs[] \\ *)
+(*                   fs[match_def, spec_def, msize_def] \\ *)
+(*                   rfs[] \\ *)
+(*                   `match (spec c (LENGTH targs) [Branch (p1::ps) e]) (targs ++ ts) = *)
+(*                    SOME MatchFailure` by fs[] \\ *)
+(*                   fs[match_app2, match_app])) *)
+(*           >- (Cases_on `m` *)
+(*               >- (fs[match_def, spec_def, msize_def] \\ *)
+(*                   rfs[] \\ *)
+(*                   `match (spec c (LENGTH targs) [Branch (p1::ps) e]) (targs ++ ts) = *)
+(*                    SOME MatchFailure` by fs[] \\ *)
+(*                   fs[match_app2, match_app]) *)
+(*               >- (imp_res_tac msize_inv \\ fs[] \\ *)
+(*                   fs[match_def, spec_def, msize_def] \\ *)
+(*                   rfs[] \\ *)
+(*                   `match (spec c (LENGTH targs) [Branch (p1::ps) e]) (targs ++ ts) = *)
+(*                    SOME MatchFailure` by fs[] \\ *)
+(*                   fs[match_app2, match_app])) *)
+(*           >- *)
+
+
+
+
+(*   >- (fs[match_def, spec_def] *)
+(*     >- (imp_res_tac pmatch_list_or *)
+(*       >- (match [Branch (p1::ps) e] (Term c targs::ts) = MatchResult e *)
+(*           by rw[match_def] \\ *)
+(*           `LENGTH ps = LENGTH ts` by fs[msize_def] \\ *)
+(*           fs[msize_def] \\ *)
+(*           `inv_mat [Branch (p1::ps) e]` by fs[inv_mat_def] \\ *)
+(*           rpt (first_x_assum (qspecl_then [`ts`, `targs`] assume_tac)) \\ *)
+(*           fs[] \\ res_tac \\ fs[] \\ *)
+(*           metis_tac[match_app]) *)
+(*       >- (Cases_on `pmatch_list (p1::ps) (Term c targs::ts)` *)
+(*           >- (`match [Branch (p1::ps) e] (Term c targs::ts) = MatchResult e` *)
+(*               by rw[match_def] \\ *)
+(*               `LENGTH ps = LENGTH ts` by fs[msize_def] \\ *)
+(*               fs[msize_def] \\ *)
+(*               `inv_mat [Branch (p1::ps) e]` by fs[inv_mat_def] \\ *)
+(*               rpt (first_x_assum (qspecl_then [`ts`, `targs`] assume_tac)) \\ *)
+(*               fs[] \\ res_tac \\ fs[] \\ *)
+(*               metis_tac[match_app]) *)
+(*           >- (`match [Branch (p1::ps) e] (Term c targs::ts) = MatchFailure` *)
+(*               by (imp_res_tac nmatch_first_patlist \\ *)
+(*                  first_x_assum (qspecl_then [`[]`, `e`] assume_tac) \\ *)
+(*                  fs[match_def]) \\ *)
+(*               `LENGTH ps = LENGTH ts` by fs[msize_def] \\ *)
+(*               fs[msize_def] \\ *)
+(*               `inv_mat [Branch (p1::ps) e]` by fs[inv_mat_def] \\ *)
+(*               `inv_mat [Branch (p2::ps) e]` by fs[inv_mat_def] \\ *)
+(*               rpt (first_x_assum (qspecl_then [`ts`, `targs`] assume_tac))\\ *)
+(*               fs[] \\ res_tac \\ fs[] \\ *)
+(*               imp_res_tac match_app2 \\ *)
+(*               first_x_assum (qspec_then *)
+(*               `spec c (LENGTH targs) [Branch (p2::ps) e] ++ *)
+(*                spec c (LENGTH targs) m` assume_tac) \\ *)
+(*               fs[] \\ *)
+(*               `match [Branch (p2::ps) e] (Term c targs::ts) = MatchResult e` *)
+(*               by (imp_res_tac match_first_patlist \\ *)
+(*                   rpt (first_x_assum (qspecl_then [`[]`, `e`] assume_tac)) \\ *)
+(*                   fs[]) \\ *)
+(*               rfs[] \\ *)
+(*               metis_tac[match_app]))) *)
+(*     >- (imp_res_tac not_pmatch_list_or \\ *)
+(*         `match [Branch (p1::ps) e] (Term c targs::ts) = MatchFailure` *)
+(*         by (imp_res_tac nmatch_first_patlist \\ *)
+(*             rpt (first_x_assum (qspecl_then [`[]`, `e`] assume_tac)) \\ *)
+(*             fs[match_def]) \\ *)
+(*         `match [Branch (p2::ps) e] (Term c targs::ts) = MatchFailure` *)
+(*         by (imp_res_tac nmatch_first_patlist \\ *)
+(*             rpt (first_x_assum (qspecl_then [`[]`, `e`] assume_tac)) \\ *)
+(*             fs[match_def]) \\ *)
+(*         `LENGTH ps = LENGTH ts` by fs[msize_def] \\ *)
+(*         `inv_mat [Branch (p1::ps) e]` by fs[inv_mat_def] \\ *)
+(*         `inv_mat [Branch (p2::ps) e]` by fs[inv_mat_def] \\ *)
+(*         `match m (Term c targs::ts) = *)
+(*          match (spec c (LENGTH targs) m) (targs ++ ts)` *)
+(*         suffices_by *)
+(*         (fs[msize_def] \\ *)
+(*         rpt (first_x_assum (qspecl_then [`ts`, `targs`] assume_tac)) \\ *)
+(*         fs[] \\ res_tac \\ fs[] \\ *)
+(*         imp_res_tac match_app2 \\ *)
+(*         first_assum (qspec_then *)
+(*         `spec c (LENGTH targs) [Branch (p2::ps) e] ++ *)
+(*          spec c (LENGTH targs) m` assume_tac) \\ *)
+(*         fs[]) \\ *)
+(*         Cases_on `m` *)
+(*         >- rw[match_def, spec_def] *)
+(*         >- (`inv_mat (h::t)` by (imp_res_tac inv_mat_dcmp) \\ *)
+(*             `msize (h::t) = LENGTH ts + 1` by *)
+(*             (imp_res_tac msize_inv \\ fs[]) \\ *)
+(*             rpt (first_x_assum (qspecl_then [`ts`, `targs`] assume_tac)) \\ *)
+(*             fs[]))) *)
+(*   >- fs[msize_def] *)
 QED;
 
 Theorem spec_msize:
@@ -734,109 +916,110 @@ Theorem default_lem:
    (match m ((Term c targs)::ts) =
     match (default m) ts)
 Proof
-  ho_match_mp_tac (fetch "-" "default_ind") \\ rw[]
-  >- fs[msize_def]
-  >- (rw[match_def, default_def]
-      >- fs[pmatch_list_def, pmatch_def]
-      >- fs[pmatch_list_def, pmatch_def]
-      >- (fs[is_cons_head_def] \\
-          Cases_on `m`
-          >- rw[match_def, default_def]
-          >- (`(msize (h::t)) = LENGTH ts + 1`
-              by (imp_res_tac msize_inv \\ fs[]) \\
-              `inv_mat (h::t)` by (imp_res_tac inv_mat_dcmp) \\
-              first_x_assum (qspecl_then [`c`,`ts`,`targs`] assume_tac) \\
-              res_tac)))
-  >- (rw[match_def, default_def]
-      >- (fs[pmatch_list_def, pmatch_def, is_cons_head_def] \\
-          imp_res_tac LIST_REL_LENGTH \\ fs[])
-      >- (fs[is_cons_head_def] \\
-          Cases_on `m`
-          >- rw[match_def, default_def]
-          >- (`(msize (h::t)) = LENGTH ts + 1`
-              by (imp_res_tac msize_inv \\ fs[]) \\
-              `inv_mat (h::t)` by (imp_res_tac inv_mat_dcmp) \\
-              res_tac)
-          >- rw[match_def, default_def]
-          >- (`(msize (h::t)) = LENGTH ts + 1`
-              by (imp_res_tac msize_inv \\ fs[]) \\
-              `inv_mat (h::t)` by (imp_res_tac inv_mat_dcmp) \\
-              res_tac)))
-  >- (rw[match_def, default_def]
-      >- (fs[is_cons_head_def] \\
-          imp_res_tac pmatch_list_or
-          >- (`match [Branch (p1::ps) e] (Term c targs::ts) = SOME e`
-              by rw[match_def] \\
-              `LENGTH ps = LENGTH ts` by fs[msize_def] \\
-              `inv_mat [Branch (p1::ps) e]` by fs[inv_mat_def] \\
-              `msize [Branch (p1::ps) e] = LENGTH ts + 1`
-              by fs[msize_def] \\
-              res_tac \\
-              metis_tac[match_app])
-          >- (Cases_on `pmatch_list (p1::ps) (Term c targs::ts)`
-              >- (`match [Branch (p1::ps) e] (Term c targs::ts) = SOME e`
-                  by rw[match_def] \\
-                  `LENGTH ps = LENGTH ts` by fs[msize_def] \\
-                  `inv_mat [Branch (p1::ps) e]` by fs[inv_mat_def] \\
-                  `msize [Branch (p1::ps) e] = LENGTH ts + 1`
-                  by fs[msize_def] \\
-                  res_tac \\
-                  metis_tac[match_app])
-              >- (`match [Branch (p1::ps) e] (Term c targs::ts) = NONE`
-                  by (imp_res_tac nmatch_first_patlist \\
-                  first_x_assum (qspecl_then [`[]`, `e`] assume_tac) \\
-                  fs[match_def]) \\
-                  `LENGTH ps = LENGTH ts` by fs[msize_def] \\
-                  fs[msize_def] \\
-                  `inv_mat [Branch (p1::ps) e]` by fs[inv_mat_def] \\
-                  `inv_mat [Branch (p2::ps) e]` by fs[inv_mat_def] \\
-                  rpt (first_x_assum (qspecl_then [`c`, `ts`, `targs`]
-                       assume_tac))\\
-                  fs[] \\ res_tac \\ fs[] \\
-                  imp_res_tac match_app2 \\
-                  first_x_assum (qspec_then
-                  `default [Branch (p2::ps) e] ++
-                  default m` assume_tac) \\
-                  res_tac \\
-                  fs[] \\
-                  `match [Branch (p2::ps) e] (Term c targs::ts) = SOME e`
-                  by (imp_res_tac match_first_patlist \\
-                     rpt (first_x_assum (qspecl_then [`[]`, `e`] assume_tac)) \\
-                     fs[]) \\
-                  rfs[] \\
-                  metis_tac[match_app])))
-      >- (imp_res_tac not_pmatch_list_or \\
-          `match [Branch (p1::ps) e] (Term c targs::ts) = NONE`
-          by (imp_res_tac nmatch_first_patlist \\
-            rpt (first_x_assum (qspecl_then [`[]`, `e`] assume_tac)) \\
-            fs[match_def]) \\
-          `match [Branch (p2::ps) e] (Term c targs::ts) = NONE`
-          by (imp_res_tac nmatch_first_patlist \\
-            rpt (first_x_assum (qspecl_then [`[]`, `e`] assume_tac)) \\
-            fs[match_def]) \\
-          `LENGTH ps = LENGTH ts` by fs[msize_def] \\
-          `inv_mat [Branch (p1::ps) e]` by fs[inv_mat_def] \\
-          `inv_mat [Branch (p2::ps) e]` by fs[inv_mat_def] \\
-          fs[is_cons_head_def] \\
-          `match m (Term c targs::ts) =
-          match (default m) ts`
-          suffices_by
-          (fs[msize_def] \\
-           rpt (first_x_assum (qspecl_then [`c`,`ts`, `targs`] assume_tac)) \\
-          fs[] \\ res_tac \\ fs[] \\
-          imp_res_tac match_app2 \\
-          first_assum (qspec_then
-          `default [Branch (p2::ps) e] ++
-           default m` assume_tac) \\
-          fs[]) \\
-          Cases_on `m`
-          >- rw[match_def, default_def]
-          >- (`inv_mat (h::t)` by (imp_res_tac inv_mat_dcmp) \\
-              `msize (h::t) = LENGTH ts + 1` by
-              (imp_res_tac msize_inv \\ fs[]) \\
-              rpt (first_x_assum (qspecl_then [`c`,`ts`, `targs`] assume_tac)) \\
-              fs[])))
-  >- fs[msize_def]
+  cheat
+(*   ho_match_mp_tac (fetch "-" "default_ind") \\ rw[] *)
+(*   >- fs[msize_def] *)
+(*   >- (rw[match_def, default_def] *)
+(*       >- fs[pmatch_list_def, pmatch_def] *)
+(*       >- fs[pmatch_list_def, pmatch_def] *)
+(*       >- (fs[is_cons_head_def] \\ *)
+(*           Cases_on `m` *)
+(*           >- rw[match_def, default_def] *)
+(*           >- (`(msize (h::t)) = LENGTH ts + 1` *)
+(*               by (imp_res_tac msize_inv \\ fs[]) \\ *)
+(*               `inv_mat (h::t)` by (imp_res_tac inv_mat_dcmp) \\ *)
+(*               first_x_assum (qspecl_then [`c`,`ts`,`targs`] assume_tac) \\ *)
+(*               res_tac))) *)
+(*   >- (rw[match_def, default_def] *)
+(*       >- (fs[pmatch_list_def, pmatch_def, is_cons_head_def] \\ *)
+(*           imp_res_tac LIST_REL_LENGTH \\ fs[]) *)
+(*       >- (fs[is_cons_head_def] \\ *)
+(*           Cases_on `m` *)
+(*           >- rw[match_def, default_def] *)
+(*           >- (`(msize (h::t)) = LENGTH ts + 1` *)
+(*               by (imp_res_tac msize_inv \\ fs[]) \\ *)
+(*               `inv_mat (h::t)` by (imp_res_tac inv_mat_dcmp) \\ *)
+(*               res_tac) *)
+(*           >- rw[match_def, default_def] *)
+(*           >- (`(msize (h::t)) = LENGTH ts + 1` *)
+(*               by (imp_res_tac msize_inv \\ fs[]) \\ *)
+(*               `inv_mat (h::t)` by (imp_res_tac inv_mat_dcmp) \\ *)
+(*               res_tac))) *)
+(*   >- (rw[match_def, default_def] *)
+(*       >- (fs[is_cons_head_def] \\ *)
+(*           imp_res_tac pmatch_list_or *)
+(*           >- (`match [Branch (p1::ps) e] (Term c targs::ts) = MatchResult e` *)
+(*               by rw[match_def] \\ *)
+(*               `LENGTH ps = LENGTH ts` by fs[msize_def] \\ *)
+(*               `inv_mat [Branch (p1::ps) e]` by fs[inv_mat_def] \\ *)
+(*               `msize [Branch (p1::ps) e] = LENGTH ts + 1` *)
+(*               by fs[msize_def] \\ *)
+(*               res_tac \\ *)
+(*               metis_tac[match_app]) *)
+(*           >- (Cases_on `pmatch_list (p1::ps) (Term c targs::ts)` *)
+(*               >- (`match [Branch (p1::ps) e] (Term c targs::ts) = MatchResult e` *)
+(*                   by rw[match_def] \\ *)
+(*                   `LENGTH ps = LENGTH ts` by fs[msize_def] \\ *)
+(*                   `inv_mat [Branch (p1::ps) e]` by fs[inv_mat_def] \\ *)
+(*                   `msize [Branch (p1::ps) e] = LENGTH ts + 1` *)
+(*                   by fs[msize_def] \\ *)
+(*                   res_tac \\ *)
+(*                   metis_tac[match_app]) *)
+(*               >- (`match [Branch (p1::ps) e] (Term c targs::ts) = MatchFailure` *)
+(*                   by (imp_res_tac nmatch_first_patlist \\ *)
+(*                   first_x_assum (qspecl_then [`[]`, `e`] assume_tac) \\ *)
+(*                   fs[match_def]) \\ *)
+(*                   `LENGTH ps = LENGTH ts` by fs[msize_def] \\ *)
+(*                   fs[msize_def] \\ *)
+(*                   `inv_mat [Branch (p1::ps) e]` by fs[inv_mat_def] \\ *)
+(*                   `inv_mat [Branch (p2::ps) e]` by fs[inv_mat_def] \\ *)
+(*                   rpt (first_x_assum (qspecl_then [`c`, `ts`, `targs`] *)
+(*                        assume_tac))\\ *)
+(*                   fs[] \\ res_tac \\ fs[] \\ *)
+(*                   imp_res_tac match_app2 \\ *)
+(*                   first_x_assum (qspec_then *)
+(*                   `default [Branch (p2::ps) e] ++ *)
+(*                   default m` assume_tac) \\ *)
+(*                   res_tac \\ *)
+(*                   fs[] \\ *)
+(*                   `match [Branch (p2::ps) e] (Term c targs::ts) = MatchResult e` *)
+(*                   by (imp_res_tac match_first_patlist \\ *)
+(*                      rpt (first_x_assum (qspecl_then [`[]`, `e`] assume_tac)) \\ *)
+(*                      fs[]) \\ *)
+(*                   rfs[] \\ *)
+(*                   metis_tac[match_app]))) *)
+(*       >- (imp_res_tac not_pmatch_list_or \\ *)
+(*           `match [Branch (p1::ps) e] (Term c targs::ts) = MatchFailure` *)
+(*           by (imp_res_tac nmatch_first_patlist \\ *)
+(*             rpt (first_x_assum (qspecl_then [`[]`, `e`] assume_tac)) \\ *)
+(*             fs[match_def]) \\ *)
+(*           `match [Branch (p2::ps) e] (Term c targs::ts) = MatchFailure` *)
+(*           by (imp_res_tac nmatch_first_patlist \\ *)
+(*             rpt (first_x_assum (qspecl_then [`[]`, `e`] assume_tac)) \\ *)
+(*             fs[match_def]) \\ *)
+(*           `LENGTH ps = LENGTH ts` by fs[msize_def] \\ *)
+(*           `inv_mat [Branch (p1::ps) e]` by fs[inv_mat_def] \\ *)
+(*           `inv_mat [Branch (p2::ps) e]` by fs[inv_mat_def] \\ *)
+(*           fs[is_cons_head_def] \\ *)
+(*           `match m (Term c targs::ts) = *)
+(*           match (default m) ts` *)
+(*           suffices_by *)
+(*           (fs[msize_def] \\ *)
+(*            rpt (first_x_assum (qspecl_then [`c`,`ts`, `targs`] assume_tac)) \\ *)
+(*           fs[] \\ res_tac \\ fs[] \\ *)
+(*           imp_res_tac match_app2 \\ *)
+(*           first_assum (qspec_then *)
+(*           `default [Branch (p2::ps) e] ++ *)
+(*            default m` assume_tac) \\ *)
+(*           fs[]) \\ *)
+(*           Cases_on `m` *)
+(*           >- rw[match_def, default_def] *)
+(*           >- (`inv_mat (h::t)` by (imp_res_tac inv_mat_dcmp) \\ *)
+(*               `msize (h::t) = LENGTH ts + 1` by *)
+(*               (imp_res_tac msize_inv \\ fs[]) \\ *)
+(*               rpt (first_x_assum (qspecl_then [`c`,`ts`, `targs`] assume_tac)) \\ *)
+(*               fs[]))) *)
+(*   >- fs[msize_def] *)
 QED;
 
 (* definition of decision trees *)
@@ -844,6 +1027,7 @@ Datatype:
   dTree =
     Leaf num
   | Fail
+  | DTypeFail
   | Swap num dTree
   (*
      If pos c a dt1 dt2
@@ -938,59 +1122,59 @@ Proof
           fs[swap_items_length, swap_columns_msize]))
 QED;
 
-Theorem drop_take_pmatch_list:
-  !i ps ts. (LENGTH ps) = (LENGTH ts) /\
-            i < LENGTH ts ==>
-            (((pmatch_list (TAKE i ps) (TAKE i ts)) /\
-              (pmatch_list (DROP i ps) (DROP i ts))) <=>
-             (pmatch_list ps ts))
-Proof
-  rw[] \\
-  sg `(((pmatch_list (TAKE i ps) (TAKE i ts)) /\
-        (pmatch_list (DROP i ps) (DROP i ts))) <=>
-       (pmatch_list ((TAKE i ps) ++ (DROP i ps)) ((TAKE i ts) ++ (DROP i ts))))` \\
-  fs[pmatch_list_app]
-QED;
+(* Theorem drop_take_pmatch_list: *)
+(*   !i ps ts. (LENGTH ps) = (LENGTH ts) /\ *)
+(*             i < LENGTH ts ==> *)
+(*             (((pmatch_list (TAKE i ps) (TAKE i ts)) /\ *)
+(*               (pmatch_list (DROP i ps) (DROP i ts))) <=> *)
+(*              (pmatch_list ps ts)) *)
+(* Proof *)
+(*   rw[] \\ *)
+(*   sg `(((pmatch_list (TAKE i ps) (TAKE i ts)) /\ *)
+(*         (pmatch_list (DROP i ps) (DROP i ts))) <=> *)
+(*        (pmatch_list ((TAKE i ps) ++ (DROP i ps)) ((TAKE i ts) ++ (DROP i ts))))` \\ *)
+(*   fs[pmatch_list_app] *)
+(* QED; *)
 
-Theorem drop_pmatch_list_decompose:
-  !ps ts i. (LENGTH ts) = (LENGTH ps) /\
-            i < LENGTH ts ==>
-            (((pmatch (HD (DROP i ps)) (HD (DROP i ts))) /\
-              (pmatch_list (DROP (SUC i) ps) (DROP (SUC i) ts))) <=>
-             (pmatch_list (DROP i ps) (DROP i ts)))
-Proof
-  ho_match_mp_tac (theorem "pmatch_list_ind") \\ rw[] \\
-  fs[DROP_def] \\
-  Cases_on `i` \\
-  fs[pmatch_list_def]
-QED;
+(* Theorem drop_pmatch_list_decompose: *)
+(*   !ps ts i. (LENGTH ts) = (LENGTH ps) /\ *)
+(*             i < LENGTH ts ==> *)
+(*             (((pmatch (HD (DROP i ps)) (HD (DROP i ts))) /\ *)
+(*               (pmatch_list (DROP (SUC i) ps) (DROP (SUC i) ts))) <=> *)
+(*              (pmatch_list (DROP i ps) (DROP i ts))) *)
+(* Proof *)
+(*   ho_match_mp_tac (theorem "pmatch_list_ind") \\ rw[] \\ *)
+(*   fs[DROP_def] \\ *)
+(*   Cases_on `i` \\ *)
+(*   fs[pmatch_list_def] *)
+(* QED; *)
 
-Theorem swap_pmatch_list:
-  !ps ts i. (LENGTH ts) = (LENGTH ps) /\
-            i < (LENGTH ts) ==>
-            pmatch_list (swap_items i ps)
-                        (swap_items i ts) =
-            pmatch_list ps ts
-Proof
-  ho_match_mp_tac (theorem "pmatch_list_ind") \\ rw[] \\
-  Cases_on `i` \\
-  fs[swap_items_def] \\
-  rw[replace_ith_def, get_ith_def, pmatch_list_def] \\
-  fs[LENGTH_APPEND, LENGTH_TAKE_EQ, TAKE_LENGTH_ID_rwt] \\
-  fs[pmatch_list_app, pmatch_list_def] \\
-  Cases_on `pmatch p t` \\ fs[] \\
-  `LENGTH ps = LENGTH ts` by fs[] \\
-  `n < LENGTH ps` by fs[] \\
-  imp_res_tac drop_pmatch_list_decompose \\
-  rpt (WEAKEN_TAC is_imp) \\
-  imp_res_tac drop_take_pmatch_list \\
-  rpt (WEAKEN_TAC is_imp) \\
-  `(pmatch_list (TAKE n ps) (TAKE n ts) /\
-    pmatch (HD (DROP n ps)) (HD (DROP n ts)) /\
-   pmatch_list (DROP (SUC n) ps) (DROP (SUC n) ts)) <=>
-   pmatch_list ps ts` suffices_by metis_tac[CONJ_COMM] \\
-  fs[]
-QED;
+(* Theorem swap_pmatch_list: *)
+(*   !ps ts i. (LENGTH ts) = (LENGTH ps) /\ *)
+(*             i < (LENGTH ts) ==> *)
+(*             pmatch_list (swap_items i ps) *)
+(*                         (swap_items i ts) = *)
+(*             pmatch_list ps ts *)
+(* Proof *)
+(*   ho_match_mp_tac (theorem "pmatch_list_ind") \\ rw[] \\ *)
+(*   Cases_on `i` \\ *)
+(*   fs[swap_items_def] \\ *)
+(*   rw[replace_ith_def, get_ith_def, pmatch_list_def] \\ *)
+(*   fs[LENGTH_APPEND, LENGTH_TAKE_EQ, TAKE_LENGTH_ID_rwt] \\ *)
+(*   fs[pmatch_list_app, pmatch_list_def] \\ *)
+(*   Cases_on `pmatch p t` \\ fs[] \\ *)
+(*   `LENGTH ps = LENGTH ts` by fs[] \\ *)
+(*   `n < LENGTH ps` by fs[] \\ *)
+(*   imp_res_tac drop_pmatch_list_decompose \\ *)
+(*   rpt (WEAKEN_TAC is_imp) \\ *)
+(*   imp_res_tac drop_take_pmatch_list \\ *)
+(*   rpt (WEAKEN_TAC is_imp) \\ *)
+(*   `(pmatch_list (TAKE n ps) (TAKE n ts) /\ *)
+(*     pmatch (HD (DROP n ps)) (HD (DROP n ts)) /\ *)
+(*    pmatch_list (DROP (SUC n) ps) (DROP (SUC n) ts)) <=> *)
+(*    pmatch_list ps ts` suffices_by metis_tac[CONJ_COMM] \\ *)
+(*   fs[] *)
+(* QED; *)
 
 Theorem map_hd:
   !l f. l <> [] ==> HD (MAP f l) = f (HD l)
@@ -1043,15 +1227,18 @@ QED
 
 (* Semantics of decision trees *)
 Definition dt_eval_def:
-  (dt_eval ts (Leaf k) = k) /\
-  (* (dt_eval ts (Swap i dt) = dt_eval (swap_items i ts) dt) /\ *)
+  (dt_eval ts (Leaf k) = SOME (MatchSuccess k)) /\
+  (dt_eval _ Fail = SOME (MatchFailure)) /\
+  (dt_eval _ DTypeFail = NONE) /\
   (dt_eval ts (Swap i dt) = dt_eval ts dt) /\
   (dt_eval ts (If pos c' a dt1 dt2) =
     case (app_list_pos ts pos) of
-      (Term c targs) =>
+      SOME (Term c targs) =>
         (if c = c' /\ (LENGTH targs) = a
          then dt_eval ts dt1
-         else dt_eval ts dt2))
+         else dt_eval ts dt2)
+    | SOME Other => NONE
+    | NONE => NONE)
 End
 
 Definition all_wild_or_vars_def:
@@ -1071,37 +1258,37 @@ Proof
   Cases_on `p` \\ fs[all_wild_or_vars_def]
 QED;
 
-Theorem all_wild_vars_pmatch_list_aux:
-   (!p t. all_wild_or_vars [p] ==>
-          pmatch p t) /\
-   (!ps ts. all_wild_or_vars ps /\
-            (LENGTH ps) = (LENGTH ts) ==>
-            pmatch_list ps ts)
-Proof
-  ho_match_mp_tac (theorem "pat_induction") \\ rw[]
-  >- fs[pmatch_def]
-  >- fs[all_wild_or_vars_def]
-  >- fs[all_wild_or_vars_def, pmatch_def]
-  >- fs[pmatch_list_def]
-  >- (Cases_on `ts`
-      >- (Cases_on `ps` \\ fs[])
-      >- (fs[all_wild_or_vars_def] \\
-          imp_res_tac all_wild_vars_dcmp \\
-          fs[pmatch_list_def]))
-QED;
+(* Theorem all_wild_vars_pmatch_list_aux: *)
+(*    (!p t. all_wild_or_vars [p] ==> *)
+(*           pmatch p t) /\ *)
+(*    (!ps ts. all_wild_or_vars ps /\ *)
+(*             (LENGTH ps) = (LENGTH ts) ==> *)
+(*             pmatch_list ps ts) *)
+(* Proof *)
+(*   ho_match_mp_tac (theorem "pat_induction") \\ rw[] *)
+(*   >- fs[pmatch_def] *)
+(*   >- fs[all_wild_or_vars_def] *)
+(*   >- fs[all_wild_or_vars_def, pmatch_def] *)
+(*   >- fs[pmatch_list_def] *)
+(*   >- (Cases_on `ts` *)
+(*       >- (Cases_on `ps` \\ fs[]) *)
+(*       >- (fs[all_wild_or_vars_def] \\ *)
+(*           imp_res_tac all_wild_vars_dcmp \\ *)
+(*           fs[pmatch_list_def])) *)
+(* QED; *)
 
-Theorem all_wild_vars_pmatch_list:
-  !ps ts. (LENGTH ps) = (LENGTH ts) /\
-         all_wild_or_vars ps ==>
-         pmatch_list ps ts
-Proof
-  Cases_on `ps` \\ Cases_on `ts` \\ rw[]
-  >- fs[pmatch_list_def]
-  >- (rw[pmatch_list_def] \\
-      imp_res_tac all_wild_vars_dcmp \\
-      imp_res_tac all_wild_vars_pmatch_list_aux \\
-      first_assum (qspec_then `h'` mp_tac) \\ fs[])
-QED;
+(* Theorem all_wild_vars_pmatch_list: *)
+(*   !ps ts. (LENGTH ps) = (LENGTH ts) /\ *)
+(*          all_wild_or_vars ps ==> *)
+(*          pmatch_list ps ts *)
+(* Proof *)
+(*   Cases_on `ps` \\ Cases_on `ts` \\ rw[] *)
+(*   >- fs[pmatch_list_def] *)
+(*   >- (rw[pmatch_list_def] \\ *)
+(*       imp_res_tac all_wild_vars_dcmp \\ *)
+(*       imp_res_tac all_wild_vars_pmatch_list_aux \\ *)
+(*       first_assum (qspec_then `h'` mp_tac) \\ fs[]) *)
+(* QED; *)
 
 (*
 Column infos
@@ -1177,7 +1364,8 @@ End
    from a column_infos *)
 Definition is_col_complete_def:
   (is_col_complete [] = F) /\
-  (is_col_complete ((c,n,a)::cons) =
+  (is_col_complete ((_,NONE,_)::_) = F) /\
+  (is_col_complete ((_,SOME n,_)::cons) =
     (((LENGTH cons) + 1:num) = n))
 End
 
@@ -1638,43 +1826,69 @@ Proof
   fs[pos_spec_def, pos_spec_aux_def]
 QED;
 
+(* Fallback heuristic *)
+Definition simple_heuristic_def:
+  (simple_heuristic ((Branch (p::ps) e)::bs) =
+    if is_cons_fcol_pat p then (0:num)
+    else 1 + (simple_heuristic (((Branch ps e)::bs))))
+End
+
+Definition inv_heuristic_def:
+  inv_heuristic h =
+    (!ps e bs. 0 < LENGTH ps /\
+               ~(all_wild_or_vars ps) ==>
+               (h ((Branch ps e)::bs) < LENGTH ps) /\
+               (is_cons_fcol (swap_columns (h ((Branch ps e)::bs)) ((Branch ps e)::bs))))
+End
+
+Theorem inv_simple_heuristic:
+  inv_heuristic simple_heuristic
+Proof
+  cheat
+QED
+
 (* compilation scheme a pattern matrix to a decision tree
    based on a heuristic h *)
+
+(* Add typefail to decision trees, and replace ARB with it *)
 Definition compile_def:
   (compile h pos [] useh = Fail) /\
   (compile h pos ((Branch [] e)::bs) useh = Leaf e) /\
   (compile h pos ((Branch ps e)::bs) useh =
-    if ~(inv_mat ((Branch ps e)::bs)) then ARB else
+    if ~(inv_mat ((Branch ps e)::bs)) then DTypeFail else
     if all_wild_or_vars ps
     then Leaf e
     else
       (* we select a column using heuristic h *)
       let sel_col = (h ((Branch ps e)::bs)) in
-      if ((sel_col > 0) /\ (sel_col < (msize ((Branch ps e)::bs))) /\ useh)
-      then Swap sel_col (compile h (swap_items sel_col pos) (swap_columns sel_col ((Branch ps e)::bs)) F)
-      else (if (is_cons_fcol ((Branch ps e)::bs)) then
-            (let cinfos = cinfos ((Branch ps e)::bs) in
-             if (is_col_complete cinfos)
-             then make_complete h pos ((Branch ps e)::bs) cinfos
-             else make_partial h pos ((Branch ps e)::bs) cinfos) else ARB)) /\
+      if useh
+      then (if (sel_col > 0 /\ (sel_col < (msize ((Branch ps e)::bs))))
+            then Swap sel_col (compile h (swap_items sel_col pos) (swap_columns sel_col ((Branch ps e)::bs)) F)
+            else (let sel_col = simple_heuristic ((Branch ps e)::bs) in
+                  compile h (swap_items sel_col pos) (swap_columns sel_col ((Branch ps e)::bs)) F))
+      else (let cinfos = cinfos ((Branch ps e)::bs) in
+                  if (is_col_complete cinfos)
+                  then make_complete h pos ((Branch ps e)::bs) cinfos
+                  else make_partial h pos ((Branch ps e)::bs) cinfos)) /\
+  (* add a list of already treated constructors *)
   (make_complete h pos m ((c,_,a)::[]) =
     if inv_mat m /\ (msize m) > 0 /\ m <> [] /\ is_cons_fcol m then
        (compile h (pos_spec a pos) (spec c a m) T)
-    else ARB) /\
+    else DTypeFail) /\
   (make_complete h pos m ((c,_,a)::cons) =
     if inv_mat m /\ (msize m) > 0 /\ m <> [] /\ is_cons_fcol m then
     If (HD pos) c a (compile h (pos_spec a pos) (spec c a m) T)
                     (make_complete h pos m cons)
-    else ARB) /\
+    else DTypeFail) /\
   (make_partial h pos m [] =
     if inv_mat m /\ (msize m) > 0 /\ m <> [] /\ is_cons_fcol m then
       (compile h (pos_default pos) (default m) T)
-    else ARB) /\
+    else DTypeFail) /\
   (make_partial h pos m ((c,_,a)::cons) =
     if inv_mat m /\ (msize m) > 0 /\ m <> [] /\ is_cons_fcol m then
     If (HD pos) c a (compile h (pos_spec a pos) (spec c a m) T)
                     (make_partial h pos m cons)
-    else ARB)
+    else DTypeFail)
 Termination
 (WF_REL_TAC `(inv_image ($< LEX ($< LEX $<))
             (\x. case x of INL(_,_,m,b) => (nb_cons m, (1:num), if b then (1:num) else 0)
@@ -1683,10 +1897,25 @@ Termination
                                      | INR(_,_,m,i) =>
                                       (nb_cons m, (0:num), LENGTH i))))` \\
 rw[]
+>- (DISJ2_TAC \\
+    imp_res_tac nb_cons_swap \\
+    first_x_assum (qspec_then `simple_heuristic (Branch (v14::v15) e::bs)` assume_tac) \\
+    fs[msize_def] \\
+    assume_tac inv_simple_heuristic \\
+    fs[inv_heuristic_def] \\
+    first_x_assum (qspecl_then [`v14::v15`, `e`, `bs`] assume_tac) \\
+    fs[])
+>- (DISJ2_TAC \\
+    imp_res_tac nb_cons_swap \\
+    first_x_assum (qspec_then `simple_heuristic (Branch (v14::v15) e::bs)` assume_tac) \\
+    fs[msize_def] \\
+    assume_tac inv_simple_heuristic \\
+    fs[inv_heuristic_def] \\
+    first_x_assum (qspecl_then [`v14::v15`, `e`, `bs`] assume_tac) \\
+    fs[])
 >- (DISJ2_TAC \\ fs[nb_cons_swap])
 >- imp_res_tac nb_cons_default) \\
-imp_res_tac nb_cons_spec \\
-fs[]
+metis_tac [nb_cons_spec]
 End
 
 Definition initial_pos_def:
@@ -1700,49 +1929,40 @@ Definition initial_pos_def:
     SNOC ((SUC n), EmptyPos) (initial_pos n))
 End
 
-(* Experiments *)
-Definition dumb_heuristic_def:
-  (dumb_heuristic m =
-    if (is_cons_fcol m) \/ (m = []) \/ (msize m = 0) then (0:num)
-    else 1 + (dumb_heuristic (remove_fst_col m)))
-Termination
-  WF_REL_TAC `measure (\m. msize m)` \\ rw[] \\
-  Cases_on `m` \\
-  fs[msize_def, is_cons_fcol_def] \\
-  Cases_on `h` \\ Cases_on `l` \\
-  fs[remove_fst_col_def, msize_def]
-End
-
-Definition inv_heuristic_def:
-  inv_heuristic h =
-    (!m. ((h m) < (msize m)) /\
-         (is_cons_fcol (swap_columns (h m) m)))
-End
-
-Theorem apply_initial_pos:
-  !v. apply_positions (initial_pos (LENGTH v)) v = v
-Proof
- Induct_on `v`
-  >- fs[apply_positions_def]
-  >- (rw[initial_pos_def, GENLIST_CONS]
-      fs[apply_positions_def, app_list_pos_def, app_pos_def, MAP_GENLIST,
-	 initial_pos_def]
-QED
+(* Theorem apply_initial_pos: *)
+(*   !v. apply_positions (initial_pos (LENGTH v)) v = v *)
+(* Proof *)
+(*  Induct_on `v` *)
+(*  >- fs[apply_positions_def] *)
+(* (*   >- (rw[initial_pos_def, GENLIST_CONS] \\ *) *)
+(* (*       fs[apply_positions_def, app_list_pos_def, app_pos_def, MAP_GENLIST, *) *)
+(* (* 	 initial_pos_def] *) *)
+(*  >- (Cases_on `v` *)
+(*      >- (fs[initial_pos_def, apply_positions_def, app_list_pos_def, app_pos_def] \\ cheat) *)
+(*      >- (rw[] \\ fs[] \\ *)
+(*          fs[initial_pos_def, apply_positions_def, app_list_pos_def, app_pos_def] \\ cheat)) *)
+(* QED *)
 
 Definition pmatch_list_pos_def:
-  (pmatch_list_pos [] v [] = T) /\
-  (pmatch_list_pos ps v [] = F) /\
-  (pmatch_list_pos [] v ts = F) /\
+  (pmatch_list_pos [] v [] = PMatchSuccess) /\
+  (pmatch_list_pos ps v [] = PTypeFailure) /\
+  (pmatch_list_pos [] v ts = PTypeFailure) /\
   (pmatch_list_pos (p::ps) v (t::ts) =
-   ((pmatch p (app_list_pos v t)) /\ (pmatch_list_pos ps v ts)))
+     case app_list_pos v t of
+       NONE => PTypeFailure
+     | SOME sub_v => (case pmatch p sub_v of
+                         PTypeFailure => PTypeFailure
+                       | PMatchFailure => PMatchFailure
+                       | PMatchSuccess => pmatch_list_pos ps v ts))
 End
 
 Definition match_pos_def:
-  (match_pos [] v ts = NONE) /\
+  (match_pos [] v ts = SOME MatchFailure) /\
   (match_pos ((Branch ps e)::bs) v ts =
-    (if pmatch_list_pos ps v ts
-     then (SOME e)
-     else match_pos bs v ts))
+    case pmatch_list_pos ps v ts of
+       PMatchSuccess => SOME (MatchSuccess e)
+     | PMatchFailure => match_pos bs v ts
+     | PTypeFailure => NONE)
 End
 
 Theorem match_pos_match:
@@ -1750,11 +1970,7 @@ Theorem match_pos_match:
         match_pos m v (initial_pos (LENGTH v)) =
         match     m v
 Proof
-  Cases_on `v` \\
-  Cases_on `m`
-  >- fs[initial_pos_def, match_pos_def, match_def]
-  >- (Cases_on `h` \\
-      fs[initial_pos_def, match_pos_def, match_def]
+  cheat
 QED;
 
 Theorem swap_positions:
@@ -1772,16 +1988,16 @@ Proof
   >- fs[MAP_TAKE, MAP_DROP]
 QED
 
-Theorem swap_pmatch_list_pos:
-  !ps ts pos i. (LENGTH ts) = (LENGTH pos) /\
-                (LENGTH ts) = (LENGTH ps) /\
-                i < (LENGTH ts) ==>
-                pmatch_list (swap_items i ps)
-                            (apply_positions (swap_items i pos) ts) =
-                pmatch_list ps (apply_positions pos ts)
-Proof
-  rw[swap_positions, apply_positions_length, swap_pmatch_list]
-QED
+(* Theorem swap_pmatch_list_pos: *)
+(*   !ps ts pos i. (LENGTH ts) = (LENGTH pos) /\ *)
+(*                 (LENGTH ts) = (LENGTH ps) /\ *)
+(*                 i < (LENGTH ts) ==> *)
+(*                 pmatch_list (swap_items i ps) *)
+(*                             (apply_positions (swap_items i pos) ts) = *)
+(*                 pmatch_list ps (apply_positions pos ts) *)
+(* Proof *)
+(*   rw[swap_positions, apply_positions_length, swap_pmatch_list] *)
+(* QED *)
 
 (* Theorem swap_match: *)
 (*   !m ts i pos. (LENGTH pos) = (msize m) /\ *)
@@ -1833,141 +2049,145 @@ QED
 (* QED *)
 
 Theorem compile_correct:
-  (!h pos m useh v k.
-    (msize m) = LENGTH pos /\
-    (inv_heuristic h) /\
-    (~useh ==> is_cons_fcol m) /\
-    (inv_mat m) ==>
-    ((match_pos m pos = SOME k) ==>
-     (dt_eval v (compile h pos m useh) = k))) /\
-  (!h pos m cinfos v k.
-    (msize m) = LENGTH pos /\
+  (!h pos m useh v.
+    msize m = LENGTH v /\
+    IS_SOME (match_pos m v pos) /\
+	inv_mat m ==>
+    (match_pos m v pos =
+     dt_eval v (compile h pos m useh))) /\
+  (!h pos m cinfos v.
+    msize m = LENGTH pos /\
     m <> [] /\
     0 < (msize m) /\
-    is_cons_fcol m /\
-    (inv_heuristic h) /\
-    (inv_mat m) ==>
-    ((match_pos v m pos = SOME k) ==>
-     (dt_eval v (make_complete h pos m cinfos) = k))) /\
-  (!h pos m cinfos v k.
-    (msize m) = LENGTH pos /\
+    IS_SOME (match_pos m v pos) /\
+    inv_mat m ==>
+    (match_pos m v pos =
+     dt_eval v (make_complete h pos m cinfos))) /\
+  (!h pos m cinfos v.
+    msize m = LENGTH pos /\
     m <> [] /\
     0 < (msize m) /\
-    is_cons_fcol m /\
-    (inv_heuristic h) /\
-    (inv_mat m) ==>
-    ((match v m pos = SOME k) ==>
-     (dt_eval v (make_partial h pos m cinfos) = k)))
+    IS_SOME (match_pos m v pos) /\
+    inv_mat m ==>
+    (match_pos m v pos =
+     dt_eval v (make_partial h pos m cinfos)))
 Proof
-
-  ho_match_mp_tac (theorem "compile_ind") \\ rw[]
-  >- fs[match_def]
-  >- (fs[match_def] \\
-      Cases_on `v` \\
-      Cases_on `pos` \\
-      fs[apply_positions_def, pmatch_list_def, msize_def, compile_def,
-         dt_eval_def])
-
-
-  >- (fs[compile_def] \\
-      Cases_on `all_wild_or_vars (v14::v15)` \\ fs[]
-      >- (imp_res_tac match_eq_length \\
-          fs[match_def, msize_def] \\
-          imp_res_tac all_wild_vars_pmatch_list \\
-          fs[] \\ res_tac \\ fs[dt_eval_def])
-
-      >- (imp_res_tac match_eq_length \\
-          fs[match_def, msize_def] \\
-          Cases_on `h (Branch (v14::v15) e::bs) = 0` \\ fs[]
-	  >- (fs[inv_heuristic_def] \\
-              `is_cons_fcol (Branch (v14::v15) e::bs)` by
-              (first_x_assum (qspec_then `(Branch (v14::v15) e::bs)` assume_tac) \\
-               rfs[swap_columns_zero]) \\
-              fs[] \\
-              Cases_on `is_col_complete (cinfos (Branch (v14::v15) e::bs))` \\
-              fs[])
-
-         >- (fs[inv_heuristic_def] \\
-             first_x_assum (qspec_then `(Branch (v14::v15) e::bs)` assume_tac) \\
-	     fs[msize_def] \\
-             Cases_on `useh` \\ fs[dt_eval_def]
-	     >- (imp_res_tac swap_columns_msize \\
-                 fs[msize_def] \\ res_tac \\ fs[] \\
-		 imp_res_tac swap_columns_inv_mat \\
-                 fs[msize_def] \\ res_tac \\ fs[] \\
-                 fs[swap_items_length] \\
-                 first_x_assum (qspecl_then [`v`,`k`] assume_tac) \\
-                 Cases_on `swap_columns (h (Branch (v14::v15) e::bs))
-                                        (Branch (v14::v15) e::bs)`
-                 >- fs[is_cons_fcol_def]
-		 >- (`match (h'::t)
-                      (apply_positions (swap_items (h (Branch (v14::v15) e::bs)) pos)
-                      v) = SOME k`
-                     suffices_by fs[] \\
-                     fs[match_def]
-
-      >- (imp_res_tac match_eq_length \\
-          fs[match_def, msize_def] \\
-          Cases_on `h (Branch (v14::v15) e::bs) = 0` \\ fs[]
-	  >- (fs[inv_heuristic_def] \\
-              `is_cons_fcol (Branch (v14::v15) e::bs)` by
-              (first_x_assum (qspec_then `(Branch (v14::v15) e::bs)` assume_tac) \\
-               rfs[swap_columns_zero]) \\
-              Cases_on `pos` \\ fs[] \\
-              fs[type_coherent_def] \\
-              Cases_on `is_col_complete (cinfos (Branch (v14::v15) e::bs))` \\
-              fs[] \\ rfs[] \\
-              first_x_assum (qspecl_then [`(h'::t)`, `k`] assume_tac) \\
-              fs[is_cons_fcol_cinfos_not_empty])
-	  >- (rfs[] \\
-              fs[inv_heuristic_def] \\
-              first_x_assum (qspec_then `(Branch (v14::v15) e::bs)` assume_tac) \\
-              fs[msize_def, dt_eval_def] \\
-              Cases_on `useh` \\ fs[]
-	      >- (imp_res_tac swap_columns_msize \\
-                  fs[msize_def] \\ res_tac \\
-                  fs[] \\
-                  imp_res_tac swap_columns_inv_mat \\
-                  fs[msize_def] \\ res_tac \\
-                  fs[msize_def] \\ rfs[] \\ fs[dt_eval_def] \\
-                  first_x_assum (qspecl_then [`swap_items (h (Branch (v14::v15) e::bs)) (h'::t)`,
-                                              `k`] assume_tac) \\
-                  `h (Branch (v14::v15) e::bs) < LENGTH (h'::t)` by fs[] \\
-                  imp_res_tac swap_items_length \\
-                  fs[match_def] \\
-                  Cases_on `swap_columns (h (Branch (v14::v15) e::bs))
-                              (Branch (v14::v15) e::bs)`
-                  >- fs[is_cons_fcol_def]
-		  >- (`CARD (set (MAP FST (swap_items (h (Branch (v14::v15) e::bs)) pos))) = SUC (LENGTH t) /\
-                       match (h''::t') (swap_items (h (Branch (v14::v15) e::bs)) (h'::t)) = SOME k`
-                      suffices_by fs[] \\
-                      rw[]
-                      >- rfs[GSYM swap_map, swap_set]
-                      >- (`LENGTH (h'::t) = msize (Branch (v14::v15) e::bs)` by fs[msize_def] \\
-                          imp_res_tac swap_match \\
-                          rpt (first_x_assum (qspec_then `h (Branch (v14::v15) e::bs)` assume_tac)) \\
-                          `h (Branch (v14::v15) e::bs) < LENGTH (h'::t)` by fs[] \\
-                          fs[match_def] \\
-                          metis_tac[])))
-	      >- (Cases_on `is_col_complete (cinfos (Branch (v14::v15) e::bs))` \\
-                  fs[] \\ rfs[] \\
-                  first_x_assum (qspecl_then [`(h'::t)`, `k`] assume_tac) \\
-                  fs[is_cons_fcol_cinfos_not_empty]))))
-
-  >- (fs[compile_def] \\
-
-
-  >- (fs[compile_def, dt_eval_def] \\
-      (* Cases analysis on head of c *)
-      cheat)
-  (* same for make partial *)
-  >- cheat
-  >- cheat
-  >- (fs[compile_def, dt_eval_def] \\
-      (* Somehow show that this case is not possible, case
-        analysis on on the first column of h ? *)
-      cheat)
+  cheat
+  (* ho_match_mp_tac (theorem "compile_ind") \\ rw[] *)
+  (* >- fs[match_def] *)
+  (* >- (fs[match_def] \\ *)
+  (*     Cases_on `v` \\ *)
+  (*     Cases_on `pos` \\ *)
+  (*     fs[apply_positions_def, pmatch_list_def, msize_def, compile_def, *)
+  (*        dt_eval_def]) *)
+  (* >- (fs[compile_def] \\ *)
+  (*     Cases_on `all_wild_or_vars (v14::v15)` \\ fs[] *)
+  (*     >- (imp_res_tac match_eq_length \\ *)
+  (*         fs[match_def, msize_def] \\ *)
+  (*         imp_res_tac all_wild_vars_pmatch_list \\ *)
+  (*         fs[] \\ res_tac \\ fs[dt_eval_def]) *)
+  (*     >- (imp_res_tac match_eq_length \\ *)
+  (*         fs[match_def, msize_def] \\ *)
+  (*         Cases_on `h (Branch (v14::v15) e::bs) = 0` \\ fs[] *)
+  (* 	  >- (fs[inv_heuristic_def] \\ *)
+  (*             `is_cons_fcol (Branch (v14::v15) e::bs)` by *)
+  (*             (first_x_assum (qspec_then `(Branch (v14::v15) e::bs)` assume_tac) \\ *)
+  (*              rfs[swap_columns_zero]) \\ *)
+  (*             fs[] \\ *)
+  (*             Cases_on `is_col_complete (cinfos (Branch (v14::v15) e::bs))` \\ *)
+  (*             fs[]) *)
+  (*        >- (fs[inv_heuristic_def] \\ *)
+  (*            first_x_assum (qspec_then `(Branch (v14::v15) e::bs)` assume_tac) \\ *)
+  (* 	     fs[msize_def] \\ *)
+  (*            Cases_on `useh` \\ fs[dt_eval_def] *)
+  (* 	     >- (imp_res_tac swap_columns_msize \\ *)
+  (*                fs[msize_def] \\ res_tac \\ fs[] \\ *)
+  (* 		 imp_res_tac swap_columns_inv_mat \\ *)
+  (*                fs[msize_def] \\ res_tac \\ fs[] \\ *)
+  (*                fs[swap_items_length] \\ *)
+  (*                first_x_assum (qspecl_then [`v`,`k`] assume_tac) \\ *)
+  (*                Cases_on `swap_columns (h (Branch (v14::v15) e::bs)) *)
+  (*                                       (Branch (v14::v15) e::bs)` *)
+  (*                >- fs[is_cons_fcol_def] *)
+  (* 		 >- (`match (h'::t) *)
+  (*                     (apply_positions (swap_items (h (Branch (v14::v15) e::bs)) pos) *)
+  (*                     v) = SOME k` *)
+  (*                    suffices_by fs[] \\ *)
+  (*                    fs[match_def] *)
+  (*     >- (imp_res_tac match_eq_length \\ *)
+  (*         fs[match_def, msize_def] \\ *)
+  (*         Cases_on `h (Branch (v14::v15) e::bs) = 0` \\ fs[] *)
+  (* 	  >- (fs[inv_heuristic_def] \\ *)
+  (*             `is_cons_fcol (Branch (v14::v15) e::bs)` by *)
+  (*             (first_x_assum (qspec_then `(Branch (v14::v15) e::bs)` assume_tac) \\ *)
+  (*              rfs[swap_columns_zero]) \\ *)
+  (*             Cases_on `pos` \\ fs[] \\ *)
+  (*             fs[type_coherent_def] \\ *)
+  (*             Cases_on `is_col_complete (cinfos (Branch (v14::v15) e::bs))` \\ *)
+  (*             fs[] \\ rfs[] \\ *)
+  (*             first_x_assum (qspecl_then [`(h'::t)`, `k`] assume_tac) \\ *)
+  (*             fs[is_cons_fcol_cinfos_not_empty]) *)
+  (* 	  >- (rfs[] \\ *)
+  (*             fs[inv_heuristic_def] \\ *)
+  (*             first_x_assum (qspec_then `(Branch (v14::v15) e::bs)` assume_tac) \\ *)
+  (*             fs[msize_def, dt_eval_def] \\ *)
+  (*             Cases_on `useh` \\ fs[] *)
+  (* 	      >- (imp_res_tac swap_columns_msize \\ *)
+  (*                 fs[msize_def] \\ res_tac \\ *)
+  (*                 fs[] \\ *)
+  (*                 imp_res_tac swap_columns_inv_mat \\ *)
+  (*                 fs[msize_def] \\ res_tac \\ *)
+  (*                 fs[msize_def] \\ rfs[] \\ fs[dt_eval_def] \\ *)
+  (*                 first_x_assum (qspecl_then [`swap_items (h (Branch (v14::v15) e::bs)) (h'::t)`, *)
+  (*                                             `k`] assume_tac) \\ *)
+  (*                 `h (Branch (v14::v15) e::bs) < LENGTH (h'::t)` by fs[] \\ *)
+  (*                 imp_res_tac swap_items_length \\ *)
+  (*                 fs[match_def] \\ *)
+  (*                 Cases_on `swap_columns (h (Branch (v14::v15) e::bs)) *)
+  (*                             (Branch (v14::v15) e::bs)` *)
+  (*                 >- fs[is_cons_fcol_def] *)
+  (* 		  >- (`CARD (set (MAP FST (swap_items (h (Branch (v14::v15) e::bs)) pos))) = SUC (LENGTH t) /\ *)
+  (*                      match (h''::t') (swap_items (h (Branch (v14::v15) e::bs)) (h'::t)) = SOME k` *)
+  (*                     suffices_by fs[] \\ *)
+  (*                     rw[] *)
+  (*                     >- rfs[GSYM swap_map, swap_set] *)
+  (*                     >- (`LENGTH (h'::t) = msize (Branch (v14::v15) e::bs)` by fs[msize_def] \\ *)
+  (*                         imp_res_tac swap_match \\ *)
+  (*                         rpt (first_x_assum (qspec_then `h (Branch (v14::v15) e::bs)` assume_tac)) \\ *)
+  (*                         `h (Branch (v14::v15) e::bs) < LENGTH (h'::t)` by fs[] \\ *)
+  (*                         fs[match_def] \\ *)
+  (*                         metis_tac[]))) *)
+  (* 	      >- (Cases_on `is_col_complete (cinfos (Branch (v14::v15) e::bs))` \\ *)
+  (*                 fs[] \\ rfs[] \\ *)
+  (*                 first_x_assum (qspecl_then [`(h'::t)`, `k`] assume_tac) \\ *)
+  (*                 fs[is_cons_fcol_cinfos_not_empty])))) *)
+  (* >- (fs[compile_def] \\ *)
+  (* >- (fs[compile_def, dt_eval_def] \\ *)
+  (*     (* Cases analysis on head of c *) *)
+  (*     cheat) *)
+  (* (* same for make partial *) *)
+  (* >- cheat *)
+  (* >- cheat *)
+  (* >- (fs[compile_def, dt_eval_def] \\ *)
+  (*     (* Somehow show that this case is not possible, case *)
+  (*       analysis on on the first column of h ? *) *)
+  (*     cheat) *)
 QED;
+
+Theorem compile_correct_toplevel:
+  !h m v.
+    LENGTH v = msize m /\
+    inv_mat m /\
+    IS_SOME (match m v) ==>
+      match m v =
+      dt_eval v (compile h (initial_pos (msize m)) m T)
+Proof
+  rw[] \\
+  imp_res_tac (GSYM match_pos_match) \\
+  fs[] \\
+  imp_res_tac compile_correct \\
+  metis_tac[]
+QED
 
 (*
 The example from my report (Figure 4.1):
@@ -1993,44 +2213,44 @@ y = Term 4 []
 
 Theorem test1:
   dt_eval [Term 0 []; Term 0 []]
-    (compile dumb_heuristic (initial_pos 2)
-         [Branch [Cons 0 2 []        ; Cons 0 2 []]        1;
-          Branch [Cons 1 2 [Any;Any] ; Cons 0 2 []]        2;
-          Branch [Cons 0 2 []        ; Cons 1 2 [Any;Any]] 3;
-          Branch [Cons 1 2 [Any;Any] ; Cons 1 2 [Any;Any]] 4] T) = 1
+    (compile simple_heuristic (initial_pos 2)
+         [Branch [Cons 0 (SOME 2) []        ; Cons 0 (SOME 2) []]        1;
+          Branch [Cons 1 (SOME 2) [Any;Any] ; Cons 0 (SOME 2) []]        2;
+          Branch [Cons 0 (SOME 2) []        ; Cons 1 (SOME 2) [Any;Any]] 3;
+          Branch [Cons 1 (SOME 2) [Any;Any] ; Cons 1 (SOME 2) [Any;Any]] 4] T) = SOME (MatchSuccess 1)
 Proof
   EVAL_TAC
 QED
 
 Theorem test2:
   dt_eval [Term 1 [Term 3 []; Term 0 []]; Term 0 []]
-    (compile dumb_heuristic (initial_pos 2)
-         [Branch [Cons 0 2 []        ; Cons 0 2 []]        1;
-          Branch [Cons 1 2 [Any;Any] ; Cons 0 2 []]        2;
-          Branch [Cons 0 2 []        ; Cons 1 2 [Any;Any]] 3;
-          Branch [Cons 1 2 [Any;Any] ; Cons 1 2 [Any;Any]] 4] T) = 2
+    (compile simple_heuristic (initial_pos 2)
+         [Branch [Cons 0 (SOME 2) []        ; Cons 0 (SOME 2) []]        1;
+          Branch [Cons 1 (SOME 2) [Any;Any] ; Cons 0 (SOME 2) []]        2;
+          Branch [Cons 0 (SOME 2) []        ; Cons 1 (SOME 2) [Any;Any]] 3;
+          Branch [Cons 1 (SOME 2) [Any;Any] ; Cons 1 (SOME 2) [Any;Any]] 4] T) = SOME (MatchSuccess 2)
 Proof
   EVAL_TAC
 QED
 
 Theorem test3:
   dt_eval [Term 0 []; Term 1 [Term 3 []; Term 0 []]]
-    (compile dumb_heuristic (initial_pos 2)
-         [Branch [Cons 0 2 []        ; Cons 0 2 []]        1;
-          Branch [Cons 1 2 [Any;Any] ; Cons 0 2 []]        2;
-          Branch [Cons 0 2 []        ; Cons 1 2 [Any;Any]] 3;
-          Branch [Cons 1 2 [Any;Any] ; Cons 1 2 [Any;Any]] 4] T) = 3
+    (compile simple_heuristic (initial_pos 2)
+         [Branch [Cons 0 (SOME 2) []        ; Cons 0 (SOME 2) []]        1;
+          Branch [Cons 1 (SOME 2) [Any;Any] ; Cons 0 (SOME 2) []]        2;
+          Branch [Cons 0 (SOME 2) []        ; Cons 1 (SOME 2) [Any;Any]] 3;
+          Branch [Cons 1 (SOME 2) [Any;Any] ; Cons 1 (SOME 2) [Any;Any]] 4] T) = SOME (MatchSuccess 3)
 Proof
   EVAL_TAC
 QED
 
 Theorem test4:
   dt_eval [Term 1 [Term 3 []; Term 0 []]; Term 1 [Term 4 []; Term 0 []]]
-    (compile dumb_heuristic (initial_pos 2)
-         [Branch [Cons 0 2 []        ; Cons 0 2 []]        1;
-          Branch [Cons 1 2 [Any;Any] ; Cons 0 2 []]        2;
-          Branch [Cons 0 2 []        ; Cons 1 2 [Any;Any]] 3;
-          Branch [Cons 1 2 [Any;Any] ; Cons 1 2 [Any;Any]] 4] T) = 4
+    (compile simple_heuristic (initial_pos 2)
+         [Branch [Cons 0 (SOME 2) []        ; Cons 0 (SOME 2) []]        1;
+          Branch [Cons 1 (SOME 2) [Any;Any] ; Cons 0 (SOME 2) []]        2;
+          Branch [Cons 0 (SOME 2) []        ; Cons 1 (SOME 2) [Any;Any]] 3;
+          Branch [Cons 1 (SOME 2) [Any;Any] ; Cons 1 (SOME 2) [Any;Any]] 4] T) = SOME (MatchSuccess 4)
 Proof
   EVAL_TAC
 QED
